Examples.lean
@@ -6,6 +6,7 @@ Authors: vvauted
 import Examples.Language.Buffer
 import Examples.Language.BufferCompiled
 import Examples.Language.Factorial
+import Examples.Language.FactorialCompiled
 import Examples.Language.Remainder
 import Examples.Language.Scalar
 import Examples.Language.ScalarCompiled
